Basic comments

theories/BlockFusion.v
@@ -1,4 +1,4 @@
-(* Block Fusion using the Block pattern *)
+(** This file defines the [BlockFusion] pattern and its semantic, and proves it is correct. *)
 
 From Vellvm Require Import Syntax ScopeTheory Semantics.
 From ITree Require Import ITree Eq.
@@ -14,18 +14,8 @@ Definition is_seq (A B: blk) := match successors A with
   | _ => false
 end.
 
-Definition BlockFusion {S} (P: Pat S) :=
+Definition BlockFusion {S} (P: Pattern S) :=
     (Block (Head P)) when (fun '(A, (B, _)) => is_seq A B).
-
-Lemma is_seq_correct:
-  forall A B, is_seq A B = true <->
-  successors A = [B.(blk_id)].
-Proof.
-  unfold is_seq. intros A B. split; intro H.
-  induction (successors A) as [|a l IHl]. discriminate. induction l.
-  apply eqb_eq in H. now subst. discriminate.
-  rewrite H. now apply eqb_eq.
-Qed.
 
 Record BlockFusion_sem A B G G': Prop := {
   EQ: G' = (remove_id B (remove_id A G));
@@ -36,27 +26,37 @@ Record BlockFusion_sem A B G G': Prop := {
   SUC: successors A = [B.(blk_id)]
 }.
 
-Theorem Pat_BlockFusion_correct {S}: forall A B G (P: Pat S) X, wf_map_cfg G ->
+Lemma is_seq_correct:
+  forall A B, is_seq A B = true <->
+  successors A = [B.(blk_id)].
+Proof.
+  unfold is_seq. intros A B. split; intro SUC.
+  induction (successors A) as [|a l REC]. discriminate. induction l.
+  apply eqb_eq in SUC. now subst. discriminate.
+  rewrite SUC. now apply eqb_eq.
+Qed.
+
+Theorem Pattern_BlockFusion_correct {S}: forall A B G (P: Pattern S) X, wf_map_cfg G ->
   (A, (B, X)) ∈ (MatchAll (BlockFusion P) G) <->
   exists G1, X ∈ (MatchAll P G1) /\ BlockFusion_sem A B G G1.
 Proof.
   intros A B G P X WFG. unfold BlockFusion. split.
   - intros H.
-    apply Pat_When_correct in H as [H SUC]. apply is_seq_correct in SUC.
-    apply Pat_Block_correct in H as [G1 [[MTA RMA WF1] H]]; trivial.
-    apply Pat_Head_correct in H as [G2 [[RMB WH2 MTB PRED] H]]; trivial.
+    apply Pattern_When_correct in H as [H SUC]. apply is_seq_correct in SUC.
+    apply Pattern_Block_correct in H as [G1 [[MTA RMA WF1] H]]; trivial.
+    apply Pattern_Head_correct in H as [G2 [[RMB WH2 MTB PRED] H]]; trivial.
     exists G2. split; trivial. subst.
-    repeat split; trivial.
+    split; trivial.
     * intro He. eapply remove_1. apply He. exists B. apply MTB.
     * eapply remove_3. apply MTB.
     * eapply add_predecessor; trivial. now apply Eempty.
   - intros [G2 [HX [EQ NEQ MTA MTB PRED SUC]]]. remember (remove_id A G) as G1.
-    apply Pat_When_correct. rewrite is_seq_correct. split; trivial.
-    apply Pat_Block_correct; trivial. exists G1.
-    repeat split; trivial. subst. now apply remove_wf_map_cfg.
-    apply Pat_Head_correct. subst. now apply remove_wf_map_cfg.
-    exists G2. subst. repeat split; trivial.
+    apply Pattern_When_correct. rewrite is_seq_correct. split; trivial.
+    apply Pattern_Block_correct; trivial. exists G1.
+    split. split; trivial. subst. now apply remove_wf_map_cfg.
+    apply Pattern_Head_correct. subst. now apply remove_wf_map_cfg.
+    exists G2. subst. split; trivial. split; trivial.
     * now repeat apply remove_wf_map_cfg.
-    * now eapply remove_2.
+    * now apply remove_2.
     * apply Eempty. apply remove_predecessor; trivial.
 Qed.
