theories/Head.v
@@ -1,3 +1,7 @@
+(** This file defines the function for the [Head] [Pattern], the semantic of the pattern,
+    and proves the correctness and completeness of that function.
+    It also provides a [predecessors] function and lemmas to reason on it. *)
+
 From Vellvm Require Import Syntax ScopeTheory Semantics.
 From ITree Require Import ITree Eq.
 Require Import FSets.FMapAVL FSets.FMapFacts.
@@ -7,7 +11,7 @@ From Pattern Require Import IdModule MapCFG.
 Import Map MapF MapF.P MapF.P.F.
 Import IdOT MapCFG.
 
-(* Head Definitions *)
+(** * This section defines the [predecessors] and [heads] functions and their semantic. *)
 
 Definition predecessors_aux (b id: bid) (bk: blk) := is_predecessor b bk.
 
@@ -21,16 +25,83 @@ Definition heads_aux (G: map_cfg) id b acc : list (blk*map_cfg) :=
 
 Definition heads (G: map_cfg): list (blk*map_cfg) := fold (heads_aux G) G [].
 
-Record head_aux_sem (G0 G G': map_cfg) b := {
+Record heads_aux_sem (G0 G G': map_cfg) b := {
   EQ: G' = (remove_id b G0);
   WF: wf_map_cfg G';
   MT: MapsTo_id b G;
   PRED: Empty (predecessors b.(blk_id) G0)
 }.
 
-Definition head_sem (G G':map_cfg) (b:blk) := head_aux_sem G G G' b.
+Definition heads_sem (G G':map_cfg) (b:blk) := heads_aux_sem G G G' b.
 
-(* Lemmas *)
+(** * This section contains lemmas used for the proof of corectness and completeness of [Head]'s semantics. *)
+
+Lemma heads_aux_sem_eq: forall G0 G G' G1 b, G' ≡ G -> heads_aux_sem G0 G G1 b <-> heads_aux_sem G0 G' G1 b.
+Proof.
+  intros GO G G' G1 b EQIV. assert (EQIV': G ≡ G') by now symmetry.
+  split; intros [EQ WF MT PRED]; repeat split; trivial;
+  eapply MapsTo_m; try apply EQIV; try apply EQIV'; try reflexivity; trivial.
+Qed.
+
+Lemma heads_aux_split: forall A B id acc G G',
+  (A, G) ∈ (heads_aux G' id B acc) -> Empty (predecessors id G') /\ A = B /\ G = remove id G' \/ (A, G) ∈ acc.
+Proof.
+  unfold heads_aux. intros A B id acc G G'.
+  remember (is_empty (predecessors id G')) as b. induction b; [intros [EQ|IN]|intros IN].
+  left. apply pair_equal_spec in EQ as [ ]. rewrite is_empty_iff. now subst.
+  all: now right.
+Qed.
+
+(** The proof of corectness and completeness of [Head]'s semantics. *)
+
+Lemma heads_aux_correct:
+  forall G G0 G' b, wf_map_cfg G -> wf_map_cfg G0 ->
+  (b, G') ∈ (fold (heads_aux G0) G []) <-> heads_aux_sem G0 G G' b.
+Proof.
+  intros G G0. apply fold_rec_bis.
+  - intros G1 G2 acc EQ REC. intros. setoid_rewrite heads_aux_sem_eq. 2:apply EQ.
+    apply REC; [apply (wf_map_cfg_eq G2)|];trivial. now symmetry.
+  - intros. split. try contradiction. intros [_ _ MT _].
+    now apply empty_mapsto_iff in MT.
+  - intros idB B acc G1 MTB NIN REC G2 A WF WF0.
+    assert (HidB: B.(blk_id) = idB). { apply WF. now apply add_1. } subst idB.
+    split.
+    * intros H. apply heads_aux_split in H as [[EM [EQA EQG]]|IN].
+      + subst. split; trivial.
+        -- now apply remove_wf_map_cfg.
+        -- now apply add_1.
+      + assert (H: (heads_aux_sem G0 G1 G2 A)). { 
+          apply REC; trivial.
+          eapply wf_map_cfg_eq. 2: { apply remove_wf_map_cfg. apply WF. }
+          symmetry. now apply remove_add_elim.
+        } destruct H as [EQ WF2 MTA PRED]. split; trivial.
+        case (eq_dec A.(blk_id) B.(blk_id)); unfold eq; [intros EQID|intros NEQID].
+        -- contradict NIN. exists A. apply eq_eq in EQID. now rewrite <- EQID.
+        -- eapply add_2. now symmetry. trivial.
+    * intros [EQ WF2 MTA PRED]. unfold heads_aux.
+      (case (eq_dec A.(blk_id) B.(blk_id)); unfold eq; [intros EQID|intros NEQID]).
+      + assert (H: A=B). {
+            eapply MapsTo_fun. apply MTA. apply eq_eq in EQID. rewrite EQID. now apply add_1.
+          } subst. remember (is_empty (predecessors B.(blk_id) G0)) as b. induction b.
+        -- now left.
+        -- apply is_empty_iff in PRED. rewrite PRED in Heqb. discriminate.
+      + assert (H: (A, G2) ∈ acc). {
+          apply REC. eapply add_wf_map_cfg. apply NIN. apply WF. trivial.
+          repeat split; trivial. eapply add_3. symmetry. apply NEQID. apply MTA.
+        } remember (is_empty (predecessors B.(blk_id) G0)) as b. induction b.
+        -- now right.
+        -- trivial.
+Qed.
+
+Lemma heads_correct:
+  forall G G' b, wf_map_cfg G ->
+  (b, G') ∈ (heads G) <-> heads_sem G G' b.
+Proof.
+  intros. now apply heads_aux_correct.
+Qed.
+
+(** * This section contains lemmas used to manipulate [predecessors] on a remove,
+      e.g. for the proofs of [BlockFusion]. *)
 
 Lemma Proper_predecessor_aux:
   forall id, Proper (eq' ==> Logic.eq ==> Logic.eq) (predecessors_aux id).
@@ -40,102 +111,36 @@ Qed.
 
 #[global] Hint Resolve Proper_predecessor_aux : core.
 
-Lemma predecessors_in: forall G id id', In id (predecessors id' G) -> In id G.
-Proof.
-  intros G id id' Hp. apply in_mapsto_iff in Hp as [B Hp]. apply in_mapsto_iff. exists B.
-  apply filter_iff in Hp as [H _]; auto.
-Qed.
-
 Lemma add_predecessor: forall (A B: blk) G G', wf_map_cfg G -> MapsTo_id A G ->
   (predecessors B.(blk_id) (remove_id A G)) ≡ G' -> successors A = [B.(blk_id)] ->
   (predecessors B.(blk_id) G) ≡ (add_id A G').
 Proof.
-  intros A B G G' Hwf HA He Hs. rewrite Equal_mapsto_iff in He. setoid_rewrite filter_iff in He; auto.
+  intros A B G G' WF MTA PRED SUC. rewrite Equal_mapsto_iff in PRED.
+  setoid_rewrite filter_iff in PRED; auto.
   apply Equal_mapsto_iff. intros idC C. setoid_rewrite filter_iff; auto. split.
-  - intros [HmC Hp]. case (eq_dec A.(blk_id) idC); unfold eq; intro Heq.
-    * apply eq_eq in Heq. assert (A=C). eapply MapsTo_fun. apply HA. now rewrite Heq.
+  - intros [MTC PREDC]. case (eq_dec A.(blk_id) idC); unfold eq; [intros EQ|intros NEQ].
+    * apply eq_eq in EQ. assert (A=C). eapply MapsTo_fun. apply MTA. now rewrite EQ.
       subst. now apply add_1.
-    * apply add_2; trivial. apply He. split;trivial. now apply remove_2.
-  - intro HC. case (eq_dec A.(blk_id) idC); unfold eq; intro Heq.
-    * apply eq_eq in Heq. assert (A=C). eapply MapsTo_fun. 2: apply HC. apply add_1. now subst.
-      subst. split; trivial. unfold predecessors_aux. unfold is_predecessor. rewrite Hs.
+    * apply add_2; trivial. apply PRED. split;trivial. now apply remove_2.
+  - intro MTC. case (eq_dec A.(blk_id) idC); unfold eq; [intros EQ|intros NEQ].
+    * apply eq_eq in EQ. assert (A=C). eapply MapsTo_fun. 2: apply MTC. apply add_1. now subst.
+      subst. split; trivial. unfold predecessors_aux. unfold is_predecessor. rewrite SUC.
       cbn. case (raw_id_eq_dec (blk_id B) (blk_id B)); auto.
     * split.
-      + eapply remove_3. apply He. eapply add_3. 2: apply HC. trivial.
-      + apply He. eapply add_3. 2: apply HC. trivial.
+      + eapply remove_3. apply PRED. eapply add_3. 2: apply MTC. trivial.
+      + apply PRED. eapply add_3. 2: apply MTC. trivial.
 Qed.
 
 Lemma remove_predecessor:
   forall id A G, wf_map_cfg G -> MapsTo_id A G -> (predecessors id G) ≡ (single A) ->
   (predecessors id (remove_id A G)) ≡ empty.
 Proof.
-  intros id A G Hwf HA Hp. rewrite Equal_mapsto_iff in Hp. setoid_rewrite filter_iff in Hp; auto.
+  intros id A G WFG MTA PRED. rewrite Equal_mapsto_iff in PRED.
+  setoid_rewrite filter_iff in PRED; auto.
   apply Equal_mapsto_iff. intros idC C. setoid_rewrite filter_iff; auto. split.
-  - intros [HmC HpC]. case (eq_dec A.(blk_id) idC); unfold eq; intro Heq.
-    * apply eq_eq in Heq. assert (A=C). eapply MapsTo_fun. apply HA. rewrite Heq. eapply remove_3.
-      apply HmC. contradict HmC. intro. eapply remove_mapsto_iff. apply H0. now subst.
-    * eapply add_3. apply Heq. apply Hp. split; trivial. eapply remove_3. apply HmC.
-  - intro HC. contradict HC. intro HC. eapply empty_mapsto_iff. apply HC.
-Qed.
-
-Lemma head_aux_sem_eq: forall G0 G G' G1 b, G' ≡ G -> head_aux_sem G0 G G1 b <-> head_aux_sem G0 G' G1 b.
-Proof.
-  intros GO G G' G1 b EQIV. assert (EQIV': G ≡ G') by now symmetry.
-  split; intros [EQ WF MT PRED]; repeat split; trivial;
-  eapply MapsTo_m; try apply EQIV; try apply EQIV'; try reflexivity; trivial.
-Qed.
-
-Lemma heads_aux_correct:
-  forall G G0 G' b, wf_map_cfg G -> wf_map_cfg G0 ->
-  (b, G') ∈ (fold (heads_aux G0) G []) <-> head_aux_sem G0 G G' b.
-Proof.
-  intros G G0. apply fold_rec_bis.
-  - intros G1 G2 a EQ REC. intros. setoid_rewrite head_aux_sem_eq. 2:apply EQ.
-    apply REC; [apply (wf_map_cfg_eq G2)|];trivial. now symmetry.
-  - intros. split. try contradiction. intros [_ _ MT _].
-    now apply empty_mapsto_iff in MT.
-  - intros idB B a G1 MTB NIN REC G2 A WF WF0.
-    assert (HidB: B.(blk_id) = idB). apply WF. now apply add_1. subst idB.
-    split.
-    * unfold heads_aux. remember (is_empty (predecessors B.(blk_id) G0)) as b. induction b. intros [EQ|IN].
-      + apply pair_equal_spec in EQ as [ ].
-        subst A G2. repeat split; trivial.
-        -- now apply remove_wf_map_cfg.
-        -- now apply add_1.
-        -- now apply is_empty_iff.
-      + assert (H: (head_aux_sem G0 G1 G2 A)). { 
-          apply REC; trivial.
-          eapply wf_map_cfg_eq. 2: {apply remove_wf_map_cfg. apply WF. } symmetry. apply remove_add_elim1; trivial.
-        } destruct H as [EQ WF2 MTA PRED]. repeat split; trivial.
-        case (eq_dec A.(blk_id) B.(blk_id)); unfold eq; [intros EQID|intros NEQID].
-        -- contradict NIN. exists A. apply eq_eq in EQID. now rewrite <- EQID.
-        -- eapply add_2. now apply neq_sym. trivial.
-      + intro IN. assert (H: (head_aux_sem G0 G1 G2 A)). { 
-          apply REC; trivial.
-          eapply wf_map_cfg_eq. 2: {apply remove_wf_map_cfg. apply WF. } symmetry. apply remove_add_elim1; trivial.
-        } destruct H as [EQ WF2 MTA PRED]. repeat split; trivial.
-        case (eq_dec A.(blk_id) B.(blk_id)); unfold eq; [intros EQID|intros NEQID].
-        -- contradict NIN. exists A. apply eq_eq in EQID. now rewrite <- EQID.
-        -- eapply add_2. now apply neq_sym. trivial.
-    * intros [EQ WF2 MTA PRED]. unfold heads_aux.
-      remember (is_empty (predecessors B.(blk_id) G0)) as b. induction b.
-      case (eq_dec A.(blk_id) B.(blk_id)); unfold eq; [intros EQID|intros NEQID].
-      + left. assert (H: A=B). {
-          eapply MapsTo_fun. apply MTA. apply eq_eq in EQID. rewrite EQID. now apply add_1.
-        } now subst.
-      + right. apply REC. eapply wf_map_cfg_add. apply NIN. apply WF. trivial.
-        repeat split; trivial. eapply add_3. apply neq_sym. apply NEQID. apply MTA.
-      + apply REC. eapply wf_map_cfg_add. apply NIN. apply WF. trivial.
-        repeat split; trivial. case (eq_dec A.(blk_id) B.(blk_id)); unfold eq; [intros EQID|intros NEQID].
-        -- assert (H: A=B). {
-            eapply MapsTo_fun. apply MTA. apply eq_eq in EQID. rewrite EQID. now apply add_1.
-          } subst A. apply is_empty_iff in PRED. rewrite PRED in Heqb. discriminate.
-        -- eapply add_3. apply neq_sym. apply NEQID. apply MTA.
-Qed.
-
-Lemma heads_correct:
-  forall G G' b, wf_map_cfg G ->
-  (b, G') ∈ (heads G) <-> head_sem G G' b.
-Proof.
-  intros. now apply heads_aux_correct.
+  - intros [MTC PREDC]. case (eq_dec A.(blk_id) idC); unfold eq; [intros EQ|intros NEQ].
+    * apply eq_eq in EQ. assert (A=C). eapply MapsTo_fun. apply MTA. rewrite EQ. eapply remove_3.
+      apply MTC. contradict MTC. intros MTC. eapply remove_mapsto_iff. apply MTC. now subst.
+    * eapply add_3. apply NEQ. apply PRED. split; trivial. eapply remove_3. apply MTC.
+  - intro MTC. contradict MTC. intro MTC. eapply empty_mapsto_iff. apply MTC.
 Qed.
