theories/Patterns.v
@@ -1,3 +1,5 @@
+(** This file defines [Pattern]s, the [MatchAll] function to interpret them, and correctness proofs. *)
+
 From Vellvm Require Import Syntax ScopeTheory Semantics.
 From ITree Require Import ITree Eq.
 From Pattern Require Import IdModule MapCFG Head Focus Block Branch.
@@ -7,22 +9,20 @@ Import ListNotations.
 Import Map MapF MapF.P MapF.P.F.
 Import IdOT MapCFG Head Focus Block Branch.
 
-(* Pattern definition *)
+(** This scetionc defines the [Pattern] type and the [MatchAll] function to interpret them. *)
 
-Inductive Pat : Type -> Type :=
-  | Graph: Pat map_cfg
-  | When: forall {S}, Pat S -> (S -> bool) -> Pat S
-  | Head: forall {S}, Pat S -> Pat (blk * S)
-  | Focus: forall {S}, Pat S -> Pat (map_cfg * S)
-  | Map: forall {S} {T}, Pat S -> (S -> T) -> Pat T
-  | Block: forall {S}, Pat S -> Pat (blk * S)
-  | Branch: forall {S}, Pat S -> Pat (blk * bid * bid * S)
+Inductive Pattern : Type -> Type :=
+  | Graph: Pattern map_cfg
+  | When: forall {S}, Pattern S -> (S -> bool) -> Pattern S
+  | Head: forall {S}, Pattern S -> Pattern (blk * S)
+  | Focus: forall {S}, Pattern S -> Pattern (map_cfg * S)
+  | Map: forall {S} {T}, Pattern S -> (S -> T) -> Pattern T
+  | Block: forall {S}, Pattern S -> Pattern (blk * S)
+  | Branch: forall {S}, Pattern S -> Pattern (blk * bid * bid * S)
 .
 
 Notation "□" := Graph.
 Notation "P 'when' b" := (When P b) (at level 45).
-
-(* Match Definitions *)
 
 Definition flat_map_r {A B C} (f : B -> list C) :=
   fix flat_map_r (l : list (A*B)) : list (A*C) :=
@@ -31,27 +31,7 @@ Definition flat_map_r {A B C} (f : B -> list C) :=
     | (a, b)::q => List.map (fun c => (a, c)) (f b)++flat_map_r q
 end.
 
-Lemma in_flat_map_r {A B C}:
-  forall (f:B->list C) (l:list (A*B)) (a:A) (c:C), (a,c) ∈ (flat_map_r f l) <->
-  exists b, (a,b) ∈ l /\ c ∈ (f b).
-Proof.
-  intro f. induction l as [|[a b] l IHl].
-  * intros. split. contradiction. intros [b [H1 H2]]. contradiction.
-  * intros a' c'. split.
-    - cbn. intro H. apply in_app_or in H as [].
-      + exists b.
-        apply Coqlib.list_in_map_inv in H as [c'' [H1 H2]].
-        apply pair_equal_spec in H1 as [].
-        subst.
-        split; trivial. left. apply pair_equal_spec. now split.
-      + assert (H': exists b0 : B, (a', b0) ∈ l /\ c' ∈ (f b0)) by now apply IHl.
-        destruct H' as [b' [H1 H2]]. exists b'. split; trivial. now right.
-    - intros [b' [[H1|H1] H2]];cbn; apply in_or_app.
-      + apply pair_equal_spec in H1 as []. subst. left. now apply in_map.
-      + right. apply IHl. now exists b'. 
-Qed.
-
-Fixpoint MatchAll {S} (P: Pat S) (g: map_cfg) : list S :=
+Fixpoint MatchAll {S} (P: Pattern S) (g: map_cfg) : list S :=
   match P with
     | □ => [g]
     | Head _ p => flat_map_r (MatchAll p) (heads g)
@@ -62,48 +42,71 @@ Fixpoint MatchAll {S} (P: Pat S) (g: map_cfg) : list S :=
     | Branch _ p => flat_map_r (MatchAll p) (branches g)
 end.
 
-(* Correction de MatchAll *)
+(** This section contains the correction (and completeness) proofs of [MatchAll].
 
-Theorem Pat_Graph_correct: forall G G', G' ∈ (MatchAll □ G) -> G' = G.
+    These proofs are done for each pattern separately.
+    They enable decontructing each atomic patterns for proof on larger ones. 
+    They mostly rely on [in_flat_map_r] and the proofs on each pattern's corresponding function, done in it's coresponding file. *)
+
+Lemma in_flat_map_r {A B C}:
+  forall (f:B->list C) (l:list (A*B)) (a:A) (c:C), (a,c) ∈ (flat_map_r f l) <->
+  exists b, (a,b) ∈ l /\ c ∈ (f b).
+Proof.
+  intro f. induction l as [|[a b] l IHl].
+  * intros. split. contradiction. intros [b [H1 H2]]. contradiction.
+  * intros a' c'. split.
+    - cbn. intro IN. apply in_app_or in IN as [IN|IN].
+      + exists b.
+        apply Coqlib.list_in_map_inv in IN as [c'' [EQ IN]].
+        apply pair_equal_spec in EQ as []. subst.
+        split; trivial. left. apply pair_equal_spec. now split.
+      + assert (H': exists b0 : B, (a', b0) ∈ l /\ c' ∈ (f b0)) by now apply IHl.
+        destruct H' as [b' [IN1 IN2]]. exists b'. split; trivial. now right.
+    - intros [b' [[EQ|IN1] IN2]];cbn; apply in_or_app.
+      + apply pair_equal_spec in EQ as []. subst. left. now apply in_map.
+      + right. apply IHl. now exists b'. 
+Qed.
+
+Theorem Pattern_Graph_correct: forall G G', G' ∈ (MatchAll □ G) -> G' = G.
 Proof.
   cbn. intros G G' H. destruct H; now destruct H.
 Qed.
 
-Theorem Pat_Head_correct {S}:
-  forall (G: map_cfg) (P: Pat S) (b:blk) s, wf_map_cfg G ->
-  (b, s) ∈ (MatchAll (Head P) G) <->
-  exists G', head_sem G G' b /\ s ∈ (MatchAll P G').
+Theorem Pattern_Head_correct {S}:
+  forall (G: map_cfg) (P: Pattern S) (b:blk) X, wf_map_cfg G ->
+  (b, X) ∈ (MatchAll (Head P) G) <->
+  exists G', heads_sem G G' b /\ X ∈ (MatchAll P G').
 Proof.
-  intros G P b s Hwf. setoid_rewrite <- heads_correct;trivial. apply in_flat_map_r.
+  intros G P b X WF. setoid_rewrite <- heads_correct;trivial. apply in_flat_map_r.
 Qed.
 
-Theorem Pat_Focus_correct {S}:
-  forall (G G1: map_cfg) (P:Pat S) s, wf_map_cfg G ->
-  (G1, s) ∈ (MatchAll (Focus P) G) <-> exists G2, focus_sem G G1 G2 /\ s ∈ (MatchAll P G2).
+Theorem Pattern_Focus_correct {S}:
+  forall (G G1: map_cfg) (P:Pattern S) X, wf_map_cfg G ->
+  (G1, X) ∈ (MatchAll (Focus P) G) <-> exists G2, focus_sem G G1 G2 /\ X ∈ (MatchAll P G2).
 Proof.
-  intros G G1 P s Hwf. setoid_rewrite <-focus_correct;trivial. apply in_flat_map_r.
+  intros G G1 P X WF. setoid_rewrite <-focus_correct;trivial. apply in_flat_map_r.
 Qed.
 
-Theorem Pat_When_correct {S}:
-  forall (P: Pat S) f x G,
-  x ∈ (MatchAll (When P f) G) <-> x ∈ (MatchAll P G) /\ f x = true.
+Theorem Pattern_When_correct {S}:
+  forall (P: Pattern S) f X G,
+  X ∈ (MatchAll (P when f) G) <-> X ∈ (MatchAll P G) /\ f X = true.
 Proof.
   intros. apply filter_In.
 Qed.
 
-Theorem Pat_Map_correct {S T}:
-  forall (P: Pat S) (f: S -> T) x G,
-  x ∈ (MatchAll (Map P f) G) <-> exists y, f y = x /\ y ∈ (MatchAll P G).
+Theorem Pattern_Map_correct {S T}:
+  forall (P: Pattern S) (f: S -> T) X G,
+  X ∈ (MatchAll (Map P f) G) <-> exists y, f y = X /\ y ∈ (MatchAll P G).
 Proof.
-  cbn. intros P f x G. split.
+  cbn. intros P f X G. split.
   - intro H. apply Coqlib.list_in_map_inv in H as [y [H1 H2]]. now exists y.
-  - intros [y [H1 H2]]. subst x. now apply in_map.
+  - intros [y [H1 H2]]. subst. now apply in_map.
 Qed.
 
-Theorem Pat_Block_correct {S}:
-  forall (G: map_cfg) (P: Pat S) (b:blk) s, wf_map_cfg G ->
-  (b, s) ∈ (MatchAll (Block P) G) <->
-  exists G', blocks_sem G G' b /\ s ∈ (MatchAll P G').
+Theorem Pattern_Block_correct {S}:
+  forall (G: map_cfg) (P: Pattern S) (b:blk) X, wf_map_cfg G ->
+  (b, X) ∈ (MatchAll (Block P) G) <->
+  exists G', blocks_sem G G' b /\ X ∈ (MatchAll P G').
 Proof.
   intros. setoid_rewrite <-blocks_correct;trivial. apply in_flat_map_r.
 Qed.
