theories/MapCFG.v
@@ -1,3 +1,5 @@
+(** This file defines an FMap that uses block_ids as keys. *)
+
 From Vellvm Require Import Syntax ScopeTheory Semantics.
 From ITree Require Import ITree Eq.
 From Pattern Require Import IdModule.
@@ -6,29 +8,28 @@ Require Import List.
 Import ListNotations.
 Import IdOT.
 
-(* cfg definition *)
-
+(** Define the Map and import the functions and lemmas to work with it. *)
 Module Map := FMapAVL.Make(IdOT).
 Module MapF := FMapFacts.OrdProperties Map.
 
 Import Map MapF MapF.P MapF.P.F.
-(* Print MapF.P. *)
 
-
-(* Notations *)
-
-Infix "∈" := List.In (at level 10).
-
-Infix "===" := eq' (at level 10).
-
-Infix "≡" := Equal (at level 10).
+(** * Notations used throughout the proofs.
+    
+  Most importantly [map_cfg]. *)
 
 Notation blk := (block dtyp).
 Notation bid := block_id.
 Notation ocfg := (ocfg dtyp).
 
 Notation map_cfg := (Map.t blk).
-Notation empty := (empty blk).
+Notation empty := (Map.empty blk).
+
+Infix "∈" := List.In (at level 10).
+
+Infix "===" := eq' (at level 10).
+
+Infix "≡" := Map.Equal (at level 10).
 
 Notation add_id b := (add b.(blk_id) b).
 Notation remove_id b := (remove b.(blk_id)).
@@ -36,157 +37,82 @@ Notation MapsTo_id b := (MapsTo b.(blk_id) b).
 
 Notation single b := (add_id b empty).
 
-(* Definitions *)
+(** * wf_map_cfg
+
+  In this section we introduce a well-formedness condition on map_cfgs,
+  which is that a block is mapped on its id.*)
 
 Definition wf_map_cfg (g: map_cfg) := forall id b, MapsTo id b g -> b.(blk_id) = id.
 
-(* Proofs *)
-
-
-Lemma add_wf_map_cfg: forall b g, wf_map_cfg g -> wf_map_cfg (add_id b g).
+Lemma add_wf_map_cfg: forall id b g, ~In id g -> wf_map_cfg (add id b g) -> wf_map_cfg g.
 Proof.
-  intros b g Hwf id a H.
-  apply add_mapsto_iff in H. destruct H as [[H1 H2]|[H1 H2]].
-  - apply eq_eq in H1. now subst.
-  - now apply Hwf.
-Qed.
-
-Lemma wf_map_cfg_add: forall id b g, ~In id g -> wf_map_cfg (add id b g) -> wf_map_cfg g.
-Proof.
-  intros idB B G HnI Hwfa idA A HA.
-  apply Hwfa. apply add_2. intro. contradict HnI.
+  intros idB B G NIN WF idA A MTA.
+  apply WF. apply add_2. intro. contradict NIN.
   exists A. eapply MapsTo_m. apply H.
   reflexivity. reflexivity. trivial. trivial.
 Qed.
 
 Lemma remove_wf_map_cfg: forall id g, wf_map_cfg g -> wf_map_cfg (remove id g).
 Proof.
-  intros b g Hwf id a H. 
-  apply remove_mapsto_iff in H as [ ]. now apply Hwf.
+  intros b g WF id a MT. 
+  apply remove_mapsto_iff in MT as [ ]. now apply WF.
 Qed.
 
 Lemma wf_map_cfg_eq: forall G G', G ≡ G' -> wf_map_cfg G -> wf_map_cfg G'.
 Proof.
-  intros G G' He Hwf. intros id b Hm.
-  apply Hwf. eapply Equal_mapsto_iff.
-  apply He. trivial.
+  intros G G' EQ WF id b MT.
+  apply WF. eapply Equal_mapsto_iff.
+  apply EQ. trivial.
 Qed.
 
 Lemma wf_map_cfg_part:
   forall G G1 G2, Partition G G1 G2 ->
   wf_map_cfg G -> wf_map_cfg G1 /\ wf_map_cfg G2.
 Proof.
-  intros G G1 G2 [Hd Hs] Hwf. split; intros id b Hm; apply Hwf; apply Hs; auto.
+  intros G G1 G2 [DIS EQ] WF. split; intros ? ? ?; apply WF; apply EQ; auto.
 Qed.
 
 Lemma wf_map_cfg_blk:
-  forall G A idA B, wf_map_cfg G -> MapsTo idA A G -> MapsTo A.(blk_id) B G -> A=B.
+  forall G A idA B, wf_map_cfg G -> MapsTo idA A G -> MapsTo A.(blk_id) B G -> A = B.
 Proof.
-  intros.
-  assert (B.(blk_id)=A.(blk_id)) by now apply H.
-  assert (A.(blk_id)=idA) by now apply H. subst.
-  eapply MapsTo_fun. apply H0. trivial.
+  intros G A idA B WF MTA MTB.
+  assert (B.(blk_id)=A.(blk_id)) by now apply WF.
+  assert (A.(blk_id)=idA) by now apply WF. subst.
+  eapply MapsTo_fun. apply MTA. trivial.
 Qed.
 
-Lemma add_remove_elim1:
-  forall id B (G: map_cfg), MapsTo id B G -> G ≡ (add id B (remove id G)).
-Proof.
-  intros id B G H. apply Equal_mapsto_iff.
-  intros k e. split; intro H'.
-  - induction (eq_dec id k) as [He|He].
-    * apply eq_eq in He. subst.
-      assert (He: B=e). eapply MapsTo_fun.
-      apply H. apply H'. subst. now apply add_1.
-    * apply add_2; trivial. now apply remove_2.
-  - apply add_mapsto_iff in H' as [[He H']| [Hne H']].
-    * apply eq_eq in He. now subst.
-    * eapply remove_3. apply H'.
-Qed.
+(** * This section contains additional manipulations on Maps. *)
 
-Lemma add_remove_elim2:
-  forall id B (G G': map_cfg), MapsTo id B G ->
-  G' ≡ (remove id G) -> G ≡ (add id B G').
-Proof.
-  intros id B G G' Hm He.
-  etransitivity. apply add_remove_elim1. apply Hm.
-  apply add_m; auto. reflexivity.
-  now symmetry.
-Qed.
-
-Lemma remove_add_elim1:
+Lemma remove_add_elim:
   forall id B (G: map_cfg), ~In id G -> G ≡ (remove id (add id B G)).
 Proof.
-  intros idB B G HnI. apply Equal_mapsto_iff. intros idA A.
-  split; intros H; case (eq_dec idA idB); intro H'.
-  - apply eq_eq in H'. subst. contradict HnI. now exists A.
-  - eapply remove_2. now apply neq_sym. apply add_2;trivial. now apply neq_sym.
-  - apply eq_eq in H'. subst. contradict H. intro H. eapply remove_1. reflexivity. exists A. apply H.
-  - eapply add_3. apply neq_sym. apply H'. eapply remove_3. apply H.
-Qed.
-
-Lemma swap_add:
-  forall id id' B B' (G : map_cfg), ~ id === id' ->
-  (add id B (add id' B' G)) ≡ (add id' B' (add id B G)).
-Proof.
-  intros id id' B B' G Hn.
-  apply Equal_mapsto_iff. intros k e.
-  induction (eq_dec k id) as [b|b]. 2: induction (eq_dec k id') as [b'|b'].
-  - apply eq_eq in b. subst.
-    split; intro H.
-    * assert (He: B=e). {
-        apply add_mapsto_iff in H as [[H1 H2]|[H1 H2]]. trivial. contradict H1. apply eq_refl.
-      } subst.
-      apply add_2. now apply neq_sym.
-      apply add_mapsto_iff. left. now split.
-    * assert (He: B=e). {
-        apply add_3 in H. apply add_mapsto_iff in H as [[H1 H2]|[H1 H2]].
-        trivial. contradict H1. reflexivity. now apply neq_sym.
-      } subst.
-      apply add_1. reflexivity.
-  - apply eq_eq in b'. subst.
-    split; intro H.
-    * assert (He: B'=e). {
-        apply add_3 in H. apply add_mapsto_iff in H as [[H1 H2]|[H1 H2]].
-        trivial. contradict H1. reflexivity. trivial.
-      } subst.
-      apply add_1. reflexivity.
-    * assert (He: B'=e). {
-        apply add_mapsto_iff in H as [[H1 H2]|[H1 H2]].
-        trivial. contradict H1. reflexivity.
-      } subst e.
-      apply add_2. trivial. apply add_1. reflexivity.
-  - split; intro H.
-    * assert (H': MapsTo k e G).
-      eapply add_3. apply neq_sym. apply b'.
-      eapply add_3. apply neq_sym. apply b. apply H.
-      apply add_2. now apply neq_sym. apply add_2. now apply neq_sym. trivial.
-    * assert (H': MapsTo k e G).
-      eapply add_3. apply neq_sym. apply b.
-      eapply add_3. apply neq_sym. apply b'. apply H.
-      apply add_2. now apply neq_sym. apply add_2. now apply neq_sym. trivial.
+  intros idB B G NIN. apply Equal_mapsto_iff. intros idA A.
+  split; intros MTA; (induction (eq_dec idA idB) as [EQ|NEQ]; [apply eq_eq in EQ; subst|]).
+  - contradict NIN. now exists A.
+  - eapply remove_2. now symmetry. apply add_2;trivial. now symmetry.
+  - contradict MTA. intro MTA. eapply remove_1. reflexivity. exists A. apply MTA.
+  - eapply add_3. symmetry. apply NEQ. eapply remove_3. apply MTA.
 Qed.
 
 Lemma Eempty: forall (G: map_cfg), Empty G <-> G ≡ empty.
 Proof.
   split.
-  - intro. apply Equal_mapsto_iff. split.
-    * intros H'. contradict H'. apply H.
-    * intros H'. now apply -> empty_mapsto_iff in H'.
-  - intros H id b H'. eapply MapsTo_m in H'; [|reflexivity|reflexivity|symmetry; apply H].
-    now apply -> empty_mapsto_iff in H'.
+  - intros EM. apply Equal_mapsto_iff. split; intros MT.
+    * contradict MT. apply EM.
+    * now apply -> empty_mapsto_iff in MT.
+  - intros EQ idB B MT. eapply MapsTo_m in MT; [|reflexivity|reflexivity|symmetry; apply EQ].
+    now apply -> empty_mapsto_iff in MT.
 Qed.
 
-Lemma in_mapsto_iff: forall (G:map_cfg) id, In id G <-> (exists B, MapsTo id B G).
+Lemma Aadd: forall (B:blk) id G G', Add id B G G' <-> G' ≡ (add id B G).
 Proof.
-  unfold In. unfold Raw.In0. now unfold MapsTo.
-Qed.
-
-Lemma filter_m: forall f (G G': map_cfg),
-  Proper (eq' ==> Logic.eq ==> Logic.eq) f -> G ≡ G' -> filter f G ≡ (filter f G').
-Proof.
-  intros ? ? ? ? H. apply Equal_mapsto_iff. setoid_rewrite filter_iff; trivial. intros idC C.
-  split; intros [H1 H2]; split; trivial; eapply MapsTo_m;
-  [reflexivity|reflexivity|symmetry;apply H|trivial|reflexivity|reflexivity|apply H|trivial].
+  intros B id G G'. unfold Add. split.
+  - intros FND. apply Equal_mapsto_iff.
+    split; intros H';apply find_mapsto_iff in H'; apply find_mapsto_iff; etransitivity; [symmetry;apply FND|trivial|apply FND|trivial].
+  - intros EQ id'. rewrite Equal_mapsto_iff in EQ. remember (find id' G') as o. induction o as [a|].
+    * symmetry. apply find_mapsto_iff. apply EQ. now apply find_mapsto_iff.
+    * symmetry. apply not_find_in_iff. symmetry in Heqo. apply not_find_in_iff in Heqo.
+      intros [A Ha]. apply EQ in Ha. contradict Heqo. now exists A. 
 Qed.
 
 Lemma eqlistA_eq: forall (l l': list (bid*blk)), eqlistA (O.eqke (elt:=blk)) l l' -> l = l'.
@@ -197,18 +123,90 @@ Proof.
   apply eq_eq in H6. now subst.
 Qed.
 
-Lemma Add_add: forall (B:blk) id G G', Add id B G G' <-> G' ≡ (add id B G).
-Proof.
-  intros B id G G'. unfold Add. split.
-  - intros H. apply Equal_mapsto_iff.
-    split; intros H';apply find_mapsto_iff in H'; apply find_mapsto_iff; etransitivity; [symmetry;apply H|trivial|apply H|trivial].
-  - intros H' id'. rewrite Equal_mapsto_iff in H'. remember (find id' G') as o. induction o as [a|].
-    * symmetry. apply find_mapsto_iff. apply H'. now apply find_mapsto_iff.
-    * symmetry. apply not_find_in_iff. symmetry in Heqo. apply not_find_in_iff in Heqo.
-      intros [A Ha]. apply H' in Ha. contradict Heqo. now exists A. 
-Qed.
-
-Lemma Below_In: forall id (G:map_cfg), Below id G -> ~ In id G.
+Lemma Below_nIn: forall id (G:map_cfg), Below id G -> ~ In id G.
 Proof.
   intros id G HB HI. eapply lt_not_eq. apply HB. apply HI. reflexivity.
 Qed.
+
+(** Bellow are lemmas that are not used anymore, they may be removed later. *)
+
+(* Lemma add_wf_map_cfg: forall b g, wf_map_cfg g -> wf_map_cfg (add_id b g).
+Proof.
+  intros b g WF id a MT.
+  apply add_mapsto_iff in MT. destruct MT as [[EQ1 EQ2]|[NEQ MT]].
+  - apply eq_eq in EQ1. now subst.
+  - now apply WF.
+Qed. *)
+
+(* Lemma add_remove_elim1:
+  forall id B (G: map_cfg), MapsTo id B G -> G ≡ (add id B (remove id G)).
+Proof.
+  intros idB B G MTB. apply Equal_mapsto_iff.
+  intros idA A. split; intro MTA.
+  - induction (eq_dec idB idA) as [EQ|NEQ].
+    * apply eq_eq in EQ. subst.
+      assert (He: B=A). eapply MapsTo_fun.
+      apply MTB. apply MTA. subst. now apply add_1.
+    * apply add_2; trivial. now apply remove_2.
+  - apply add_mapsto_iff in MTA as [[EQ1 EQ2]| [NEQ MTA]].
+    * apply eq_eq in EQ1. now subst.
+    * eapply remove_3. apply MTA.
+Qed. *)
+
+(* Lemma add_remove_elim2:
+  forall id B (G G': map_cfg), MapsTo id B G ->
+  G' ≡ (remove id G) -> G ≡ (add id B G').
+Proof.
+  intros id B G G' EQR EQA.
+  etransitivity. apply add_remove_elim1. apply EQR.
+  apply add_m; auto. reflexivity.
+  now symmetry.
+Qed. *)
+
+(* Lemma swap_add:
+  forall idB idC B C (G : map_cfg), ~ idB === idC ->
+  (add idB B (add idC C G)) ≡ (add idC C (add idB B G)).
+Proof.
+  intros idB idC B C G NEQ.
+  apply Equal_mapsto_iff. intros idA A.
+  induction (eq_dec idA idB) as [EQB|NEB]. 2: induction (eq_dec idA idC) as [EQC|NEQC].
+  - apply eq_eq in EQB. subst.
+    split; intro MT.
+    * assert (H: B=A). {
+        apply add_mapsto_iff in MT as [[EQ1 EQ2]| [NEQ' MTA]]. trivial. contradict NEQ'. apply eq_refl.
+      } subst.
+      apply add_2. now symmetry.
+      apply add_mapsto_iff. left. now split.
+    * assert (H: B=A). {
+        apply add_3 in MT. apply add_mapsto_iff in MT as [[EQ1 EQ2]| [NEQ' MTA]].
+        trivial. contradict NEQ'. reflexivity. now symmetry.
+      } subst.
+      apply add_1. reflexivity.
+  - apply eq_eq in EQC. subst.
+    split; intro MT.
+    * assert (H: C=A). {
+        apply add_3 in MT. apply add_mapsto_iff in MT as [[EQ1 EQ2]| [NEQ' MTA]].
+        trivial. contradict NEQ'. reflexivity. trivial.
+      } subst.
+      apply add_1. reflexivity.
+    * assert (H: C=A). {
+        apply add_mapsto_iff in MT as [[EQ1 EQ2]| [NEQ' MTA]].
+        trivial. contradict NEQ'. reflexivity.
+      } subst.
+      apply add_2. trivial. apply add_1. reflexivity.
+  - split; intro MT.
+    * assert (H': MapsTo idA A G).
+      eapply add_3. 2:eapply add_3. 3:apply MT. now symmetry. now symmetry. trivial.
+      apply add_2. now symmetry. apply add_2. now symmetry. trivial.
+    * assert (H': MapsTo idA A G).
+      eapply add_3. 2:eapply add_3. 3:apply MT. now symmetry. now symmetry. trivial.
+      apply add_2. now symmetry. apply add_2. now symmetry. trivial.
+Qed. *)
+
+(* Lemma filter_m: forall f (G G': map_cfg),
+  Proper (eq' ==> Logic.eq ==> Logic.eq) f -> G ≡ G' -> filter f G ≡ (filter f G').
+Proof.
+  intros ? ? ? ? EQ. apply Equal_mapsto_iff. setoid_rewrite filter_iff; trivial. intros idC C.
+  split; intros [H1 H2]; split; trivial; eapply MapsTo_m;
+  [reflexivity|reflexivity|symmetry;apply EQ|trivial|reflexivity|reflexivity|apply EQ|trivial].
+Qed. *)
